fstar-helpers/fstar-bitvec/BitVec.Intrinsics.fst
@@ -10,7 +10,9 @@ let mk_bv #len (f: (i:nat{i < len}) -> bit) = on (i:nat {i < len}) f
 
 let mm256_slli_epi16 (shift: nat {shift <= 16}) (vec: bit_vec 256): bit_vec 256
   = mk_bv (fun i -> let nth_bit = i % 16 in
-                 if i >= shift then vec (i - shift) else 0)
+                 if nth_bit >= shift 
+                 then vec (i - shift)
+                 else 0)
 
 let mm256_castsi256_si128 (vec: bit_vec 256): bit_vec 128
   = mk_bv (fun i -> vec i)
@@ -39,24 +41,71 @@ private let saturate8 (v: bit_vec 16): bit_vec 8
            else v i
     )
 
+let mm_movemask_epi8_bv (a: bit_vec 128): bit_vec 128
+  = mk_bv (fun j ->
+             if j < 16
+             then a ((j * 8) + 7)
+             else 0
+          )
+
+let mm_movemask_epi8 (a: bit_vec 128): i32
+  = bit_vec_to_int_t 32 (mk_bv (fun i -> mm_movemask_epi8_bv a i))
+
+let mm256_set_epi16 (x0 x1 x2 x3 x4 x5 x6 x7 x8 x9 x10 x11 x12 x13 x14 x15: i16)
+  : bit_vec 256
+  = mk_bv (fun i ->
+      let offset = i % 16 in
+      match i / 16 with
+      |  0 -> get_bit  x0 (sz offset)
+      |  1 -> get_bit  x1 (sz offset)
+      |  2 -> get_bit  x2 (sz offset)
+      |  3 -> get_bit  x3 (sz offset)
+      |  4 -> get_bit  x4 (sz offset)
+      |  5 -> get_bit  x5 (sz offset)
+      |  6 -> get_bit  x6 (sz offset)
+      |  7 -> get_bit  x7 (sz offset)
+      |  8 -> get_bit  x8 (sz offset)
+      |  9 -> get_bit  x9 (sz offset)
+      | 10 -> get_bit x10 (sz offset)
+      | 11 -> get_bit x11 (sz offset)
+      | 12 -> get_bit x12 (sz offset)
+      | 13 -> get_bit x13 (sz offset)
+      | 14 -> get_bit x14 (sz offset)
+      | 15 -> get_bit x15 (sz offset)
+    )
+
 open FStar.Stubs.Tactics.V2.Builtins
+open FStar.Stubs.Tactics.V2
+open FStar.Tactics.V2.Derived
+open FStar.Tactics.V2
 
 let rec bv_to_string #len (bv: bit_vec len): string
   = if len = 0 then ""
                else string_of_int (bv (len - 1)) 
                   ^ bv_to_string #(len - 1) (mk_bv (fun i -> bv i))
 
+let bv_of_string #len (s: string): Tac (bit_vec len)
+  = let l = FStar.String.list_of_string s 
+          |> filter (function ' ' | '\n' -> false | _ -> true)
+          |> map #_ #bit (function '1' -> 1 <: bit | '0' -> 0 | c -> fail ("expected 0 or 1, got [" ^ String.string_of_char c ^ "]")) in
+    if FStar.List.Tot.length l = len
+    then mk_bv (fun (i: nat {i < len}) -> List.Tot.index l i)
+    else fail ("expected a bv of length " ^ string_of_int len ^ ", got a bv of length " ^ string_of_int (FStar.List.Tot.length l))
 
+let call_native_intrinsic' #ilen name raw_args (bitvecs: list (bit_vec ilen)) : Tac string =
+  let bitvecs = List.Tot.map bv_to_string bitvecs in
+  let args = List.Tot.append raw_args bitvecs in
+  let result = launch_process "bash" ("/tmp/run.sh"::name::args) "" in
+  print ("process stdout is [" ^ result ^ "]");
+  FStar.String.list_of_string result
+    |> filter (function ' ' | '\n' -> false | _ -> true)
+    |> String.string_of_list
 
-// let _ = assert True by (
-//     let s = launch_process "bit-playground" [
-//       "mm256_slli_epi16";
-//       "15";
-//       "0100000000000000000000000000000000000000000000000000000000000000000000000000000000000000000000000000000000000000000000000000000000000000000000000000000000000000000000000000000000000000000000000000000000000000000000000000000000000000000000000000000000000000";
-//     ] "" in
-//     print s
-//   )
+let call_native_intrinsic #ilen olen name raw_args (bitvecs: list (bit_vec ilen)) : Tac (bit_vec olen) =
+  bv_of_string (call_native_intrinsic' #ilen name raw_args bitvecs)
 
+let random_bv len: Tac (bit_vec len) 
+  = call_native_intrinsic #1 _ "rand" [string_of_int len] []
 
 let mm_packs_epi16 (a b: bit_vec 128): bit_vec 128
   = mk_bv (fun i ->
@@ -68,13 +117,5 @@ let mm_packs_epi16 (a b: bit_vec 128): bit_vec 128
       saturate8 (mk_bv (fun j -> vec (offset16 + j))) (i - offset8)
     )
 
-let mm_movemask_epi8_bv (a: bit_vec 128): bit_vec 128
-  = mk_bv (fun j ->
-             if j < 16
-             then a ((j * 8) + 7)
-             else 0
-          )
-
-let mm_movemask_epi8 (a: bit_vec 128): i32
-  = bit_vec_to_int_t 32 (mk_bv (fun i -> mm_movemask_epi8_bv a i))
-
+let tassert (x: bool): Tac unit
+  = if x then () else fail "tassert"
